src/lowparse/LowParse.Spec.Combinators.fst
@@ -693,6 +693,28 @@ let serialize_synth_eq
 = ()
 
 abstract
+let serialize_synth_eq'
+  (#k: parser_kind)
+  (#t1: Type0)
+  (#t2: Type0)
+  (p1: parser k t1)
+  (f2: t1 -> GTot t2)
+  (s1: serializer p1)
+  (g1: t2 -> GTot t1)
+  (u: unit {
+    synth_inverse f2 g1 /\
+    synth_injective f2
+  })
+  (x: t2)
+  (y1: bytes)
+  (q1: squash (y1 == serialize (serialize_synth p1 f2 s1 g1 u) x))
+  (y2: bytes)
+  (q2: squash (y2 == serialize s1 (g1 x)))
+: Lemma
+  (ensures (y1 == y2))
+= serialize_synth_eq p1 f2 s1 g1 u x
+
+abstract
 let serialize_synth_upd_chain
   (#k: parser_kind)
   (#t1: Type0)
